Cs2120f24/Lectures/03_natural_number_arithmetic/notes.lean
@@ -1,0 +1,35 @@
+/-!
+## The Nat Type and its Value Constructors
+
+UNDER CONSTRUCTION: NO GUARANTEES
+
+Nat is a type, the terms of which have been designed for the
+express purpose of representing natural numbers, the infinite
+set of whole numbers from zero on up by ones.
+-/
+
+
+/-!
+Here is the intended correspondence:
+
+0   Nat.zero
+1   Nat.succ Nat.zero
+2   Nat.succ (Nat.succ Nat.zero)
+3   Nat.succ (Nat.succ (Nat.succ Nat.zero))
+etc
+
+The *constant* term, Nat.zero, is taken to represent the natural
+number, 0. Lean provides the notation, 0, for Nat.zero, and it is
+important to use 0 instead of Nat.zero to take advantage of some
+Lean capabilities when we get further into proofs.
+
+The second, one-argument constructor, Nat.succ : Nat → Nat, takes
+any natural number, let's call it n', as an argument, and yields the
+term, (Nat.succ n'), which we will take to represent one more than n'.
+We will call one more than n'the *successor* of n'
+
+When writing Lean definitions it's best to write n' + 1 rather
+than (Nat.succ n') to take advantage of certain automations later
+on. Using the notations 0 and _ + 1 also makes definitions easier
+to read for most people.
+-/
