Cs2120f24/Library/natArithmetic/semantics.lean
@@ -2,9 +2,13 @@ import «cs2120f24».Library.natArithmetic.syntax
 
 namespace cs2120f24.arith
 
-#check Nat
+#check ArithExpr
 
--- type of interpretation of arithmetic variables
-def arith_var_interp := natVar → Nat
+-- Semantics (incomplete, to be finished in homework)
+def arithEval : ArithExpr → (ArithVar → Nat) → Nat
+| ArithExpr.lit (fromNat : Nat),      i =>  fromNat
+| ArithExpr.var (fromVar : ArithVar), i => i fromVar
+| ArithExpr.unOp op e,                i => 0
+| ArithExpr.binOp op e1 e2,           i => 0
 
 end cs2120f24.arith
