Cs2120f24/Library/propLogic/models_counterexamples.lean
@@ -7,19 +7,6 @@ import Cs2120f24.Lectures.«02_prop_logic».formal.utilities
 namespace cs2120f24
 
 /-!
-As a final chapter in our unit on propositional logic, we
-now present the concepts of models and counter-examples.
-
-Given a proposition (PLExpr), e, and an interpretation for
-the variables in e, we can apply our semantic evalation
-function, evalPLExpr, to e and i, to compute the truth
-value of the proposition, e, when understood to be about
-the "situation" or "world" or "state of affairs" described
-by i.
--/
-
-
-/-!
 MODELS
 
 A model is an interpretation that makes a proposition true.
@@ -27,7 +14,10 @@ A "SAT solver" (like is_sat) returns true if  there's at least
 one such interpretation. A function that actually returns such
 an interpretation (not just a Boolean value) is called a model
 finder. A related problem is to find *all* models of a given
-proposition. How would you do that?
+proposition. How would you do that? You can use the function,
+findModels. It returns a list of all models of a given expression
+(but will run out of space or time quickly as the problem size
+grows).
 -/
 
 def findModels (e : PLExpr) : List BoolInterp :=
@@ -35,6 +25,11 @@ def findModels (e : PLExpr) : List BoolInterp :=
     (fun i => evalPLExpr e i = true) -- given i, true iff i is model of e
     (listInterpsFromExpr e)
 
+/-!
+Finds all models, if any, and returns either none, if there
+wasn't one, or some m, where m is firstin the returned list
+of models.
+-/
 def findModel :  PLExpr → Option BoolInterp
 | e =>
   let ms := findModels e
@@ -45,22 +40,12 @@ def findModel :  PLExpr → Option BoolInterp
 /-
 COUNTEREXAMPLES
 
-A counterexample is an interpretation that makes a proposition
-false. If you write a *specification*, S, about a system in the
-form of a proposition that should be true of all possible system
-behaviors, you'd like to know if there are any behaviors that
-do *not* satisfy the specification. Such a behavior would be
-a *counterexample* to the specification. So how might we put
-together a method for finding a counterexample if there is one?
+We return all counterexamples, or one if there was one, for
+any given expression. These operations find models of the negation
+of the given expression, which amount to counterexamples for it.
 -/
 
 def findCounterexamples (e : PLExpr) : List BoolInterp := findModels ¬e
 def findCounterexample (e : PLExpr) : Option BoolInterp := findModel ¬e
 
-/-!
-These functions use types you don't yet know about: namely List and Option.
-You should understand lists intuitively from CS1. You can think of an option
-as a list of length either zero (called none) or one (called some e), where
-e the specific value in the length-one list of values (an interpertation).
--/
 end cs2120f24
