MyWork/99_snippets/cuts.lean
@@ -29,3 +29,41 @@ The constructors of a type *introduce* new instances/values of that type
 into the discussion. These are akin to the introduction and elimination
 inference rules discussion elsewhere in this class.
 -/
+
+
+-- --------------
+
+
+
+
+/- -------------
+
+-- arithmetic variables
+structure natVar where
+  (index : Nat)
+
+-- unary arithmetic operators (here increment, decrement)
+inductive arith_UnOp where
+| fac
+
+-- binary arithemtic operators (here +, -, and *)
+inductive arith_BinOp where
+| add
+| sub
+| mul
+
+-- abstract syntax
+inductive arithExpr
+| lit (n : Nat)
+| var (v : natVar)
+| UnOp (op : arith_UnOp) (e : arithExpr)
+| BinOp (op : arith_BinOp) (e1 e2 : arithExpr)
+
+-- concrete syntax
+notation " { " v " } " => arithExpr.var v
+notation:max "++" n => arithExpr.UnOp arith_UnOp.inc n
+notation:max "--" n => arithExpr.UnOp arith_UnOp.dec n
+notation e1 "+" e2 => arithExpr.BinOp arith_BinOp.add e1 e2
+notation e1 "-" e2 => arithExpr.BinOp arith_BinOp.sub e1 e2
+notation e1 "*" e2 => arithExpr.BinOp arith_BinOp.mul e1 e2
+-/
