MyWork/99_snippets/example.lean
@@ -1,0 +1,18 @@
+import «Cs2120f24».Library.natArithmetic.semantics
+
+namespace cs2120f24.arith
+
+-- variable expression from variable with index 0
+def X := { ⟨ 0 ⟩ }
+
+-- interpretation: every variable goes to 5
+def i0 : ArithVar → Nat := fun _ => 5
+
+-- what is the value of X under i0?
+#eval arithEval X i0    -- expect 5
+
+-- extra sauce: what does this show?
+-- put it in mathy English
+#eval arithEval {⟨9⟩} i0
+
+end cs2120f24.arith
