MyWork/deduction.lean
@@ -1,0 +1,156 @@
+import Cs2120f24.Lectures.«02_prop_logic».formal.properties
+import Cs2120f24.Lectures.«02_prop_logic».formal.interpretation
+import Cs2120f24.Lectures.«02_prop_logic».formal.semantics
+import Cs2120f24.Lectures.«02_prop_logic».formal.truth_table
+import Cs2120f24.Lectures.«02_prop_logic».formal.utilities
+
+
+/-!
+- Accept certain "rules of inference/reasoning" as valid
+- For PL: accept the *semantically valid* facts from HW1
+
+Goal is to show proposition true under given assumptions
+
+- set-up problem as a sequent: *assumptions ⊢ goal*
+- apply rules to transform sequent until no goals remain
+-/
+
+/-!
+AXIOMS
+
+-- And
+and_intro :=          S ⇒ R ⇒ S ∧ R
+and_elim_left :=      S ∧ R ⇒ S
+and_elim_right :=     S ∧ R ⇒ R
+
+-- Or
+or_intro_left :=      S ⇒ S ∨ R
+or_intro_right :=     R ⇒ S ∨ R
+or_elim :=            R ∨ S ⇒ (R ⇒ W) ⇒ (S ⇒ W) ⇒ W
+
+-- Negation
+not_intro :=          (S ⇒ ⊥) ⇒ ¬S
+not_elim :=           ¬¬S ⇒ S
+
+-- Implies
+imp_intro :=          S ⇒ W ⇒ (S ⇒ W)
+imp_elim :=           (S ⇒ W) ⇒ S ⇒ W
+
+-- Equivalence
+equiv_intro :=        (S ⇒ W) ⇒ (W ⇒ S) ⇒ (S ↔ W)
+equiv_elim_left :=    (S ↔ W) ⇒ (S ⇒ W)
+equiv_elim_right :=   (S ↔ W) ⇒ (W ⇒ S)
+-/
+
+
+/-!
+Example #1: and_intro
+
+Suppose R and S are true; show R ∧ S is then true.
+
+First, set up problem as sequent:
+
+R, S ⊢ R ∧ S
+
+Now use the axioms or any other validated propositions to derive
+the truth of the goal proposition.
+
+We know what we need. What do we have to work with? The assumptions!
+
+- "apply" the and_intro "inference rule" to R and S to derive the truth of R ∧ S
+- R ∧ S can now be removed as a goal and added to the context leaving nothing left to prove
+
+R, S, R ∧ S ⊢ {}
+
+-/
+
+/-!
+Example #2: and_intro
+
+Problem: Show that P ∧ Q is valid.
+
+There are no assumptions in this problem, just the goal.
+This is the typical starting point for proving any kind
+of proposition. We know that this goal proposition is not
+valid *semantically*. Let's see where we get stuck trying
+to prove it by natural deduction.
+
+⊢ P ∧ Q
+
+The only way we ultimately have to derive the truth of P ∧ Q
+is to apply and_intro to the truth of P and the truth of Q.
+The problem is that we haven't either assumed or shown that
+either P or Q is true.
+
+The best we can do is to *apply and_intro to arguments that we
+don't yet have *but promise to deliver in the future*. We write
+that like this: and_intro _ _. If we *had* the arguments that
+we need (truth of P, and truth of Q) we'd be done, as and_intro
+applied to them would derive the truth of P ∧ Q, which is what
+we want. But we don't have these argument values and so we are
+left is with two new goals: derive the truth of P, and derive
+the truth of Q.
+
+⊢ P
+⊢ Q
+
+Sadly we have no additional information to derive the truth of
+either of them, We're stuck and can't complete the derivation.
+-/
+
+/-!
+Example 3: But there's something really interesting going on
+there. Applying a rule to the *missing arguments* left us with
+two new sub-goals.
+
+Let's return to the first problem and see how this works out.
+
+Show R, S ⊢ R ∧ S.
+
+First apply "and_intro _ _" to construct a proof of R ∧ S but
+with the two sub-goals left to prove: R, and S, respectively.
+Here are the resulting sequents.
+
+R, S ⊢ R
+R, S ⊢ S
+
+Second, in each of these cases, the goal that's left to prove
+is already *assumed* to be true, these two goals, and there is
+nothing left to prove.
+
+R, S ⊢ {}
+R, S ⊢ {}
+
+Example #1 is an example of a "bottom-up" proof, where we apply
+rules to already known facts to derive new ones. This example is
+a "top-down" proof, where we provided a *compelete* proof but for
+certain remaining "holes," which become new "smaller" sub-goals.
+Once we "prove/construct" each of the arguments, the application
+of the top-level rule, and_intro, can complete, finishing off the
+proof.
+-/
+
+/-!
+Example #4: and_elim
+
+Suppose R ∧ S is true. Show that R is true.
+
+Sequent: R ∧ S ⊢ R
+
+apply *and_elim_left* to R ∧ S to derive R, add it to the context
+and remove it from the context
+
+R ∧ S, R ⊢ R
+
+Now R is accepted as true and can be removed as a goal. We can say
+it's already an assumption, so the proof is complete.
+
+R ∧ S, R ⊢ ⊤    -- QED
+-/
+
+
+/-!
+affirm_disjunct :=    (W ∨ S) ⇒ W ⇒ ¬S
+affirm_consequent :=  (S ⇒ W) ⇒ W ⇒ S
+deny_antecedent :=    (S ⇒ W) ⇒ ¬S ⇒ ¬W
+-/
