MyWork/homework_keys/key_02_prop_logic.lean
@@ -1,0 +1,196 @@
+import «Cs2120f24».Lectures.«02_prop_logic».formal.syntax
+import «Cs2120f24».Lectures.«02_prop_logic».formal.semantics
+import «Cs2120f24».Lectures.«02_prop_logic».formal.properties
+
+/-!
+CS 2120-002 F24 Homework #1: Propositional Logic
+-/
+
+namespace cs2120f24
+open PLExpr
+
+
+/-!
+First, we define three propositional variables: Wet, Rain, and
+Sprink, following the exmaple presented in class, with shorter
+but still suggestive variable names, for ease of reading and
+writing propositional logic expressions -- aka "propositions."
+
+Your first task is to be sure you understand the notation we're
+using. Consider the first line below:
+
+def wet : PLExpr := {⟨0⟩}.
+
+We break that down here. *Study this material.* It's not very
+difficult, and you really do need to understand this notation
+easily going forward.
+
+def       -- keyword to bind name (wet) to a value (here {⟨0⟩})
+: PLExpr  -- defines the type of value to be bound (here, PLExpr)
+:=        -- separates "variable type declaration" from value
+⟨ 0 ⟩     -- Lean-defined shorthand for (BoolExpr.mk 0)
+{ ... }   -- our concrete syntax for PLExpr.var_expr.mk
+
+The parts here that might cause some conflusion are ⟨ _ ⟩ and
+{ _ }. First, the funny angle brackets are not on your keyboard;
+they are special characters you need to enter in VSCode using
+\< and \>. Enter these strings then a space to get these
+characters. Second, a "structure" type in Lean is an inductive
+type with *just one constructor* that defaults in name to "mk".
+An example is BoolVar.mk. Rather than typing that constructor
+expression each time you want a new value *of *any* structure
+type), you can use this this angle bracket notation instead.
+Lean just has to be able to figure out from context what type
+of object is needed so that it can translate ⟨ ⟩ into a call
+to the "mk" constructor for the right structure type.
+
+Next, the {...} notation is a concrete syntax notation that we
+ourselves have defined (in syntax.lean) for PLExpr.var_expr. It
+in turn expects a BoolVar argument, which is how Lean know what
+constructor to use for the ⟨_⟩ notation: namely BoolVar.mk.
+
+The reading should help with the ⟨_⟩ notation. And you should be
+able to understand how we've defined { } as a concrete syntax in
+syntax.lean.
+-/
+
+
+def wet : PLExpr := {⟨0⟩}
+def rain : PLExpr := {⟨1⟩}
+def sprink : PLExpr := {⟨2⟩}
+
+
+/-!
+ENGLISH TO FORMAL PROPOSITIONAL LOGIC
+
+Problem #1: 50 points. Using the variable names, wet, rain,
+and sprink, write propositional logic expressions for each of
+the given propositions (expressions) written in natural language.
+For example, "it's raining and the springler is running" would be
+(rain ∧ sprink). Wtite your expressions in place of the sorrys.
+
+Once you've written your expression, add a line of "code" to
+check your expressions for *validity*. Then, if the expression
+is *not* valid, in English explain very briefly a situation in
+which the proposition is not true. For example, you know that
+raining ∧ sprinking is not valid, and in this case it would be
+ok to write "if it's not raining then this proposition is false"
+-/
+
+/-!
+A. It's raining and the sprinkler is running (free 5 points!)
+-/
+def formal_0 : PLExpr := sorry
+
+
+/-!
+B. If it's raining then it's raining or the sprinkler's running.
+Rememver to use \=> for the implies "connective" (expression
+builder).
+-/
+def formal_1  : PLExpr := sorry
+
+/-!
+C. If the sprinkler's running then it's raining or it's sprinkling.
+-/
+def formal_2  : PLExpr := sorry
+
+/-!
+D. Whenever it's raining the streets are wet. You can express the same
+idea as "if it's raining then the streets are wet." Be sure you see that
+these two English-language phrases mean the same thing. You will want to
+use the "whenever" form sometimes and the "if then" form sometimes when
+writing logic in English.
+-/
+def formal_3  : PLExpr := sorry
+
+/-!
+E. Whenever the sprinkler's running the streets are wet.
+-/
+def formal_4 : PLExpr := sorry
+
+/-!
+Here's an example, from class, of a proposition built up in
+part from several smaller *implies* propositions. This is a
+reminder to help you with any similar cases that follow.
+
+If it's raining or the sprinkler's running, then if whenever
+it's raining then the streets are wet, then if whenever the
+sprinkler's running then the streets are wet, then the streets
+are wet.
+
+Add a check for the validity of this expression. The *example*
+keyword in Lean asks Lean to check a term without binding a
+name to it.
+-/
+example  : PLExpr :=
+  rain ∨ sprink ⇒
+  (rain ⇒ wet) ⇒
+  (sprink ⇒ wet) ⇒
+  wet
+
+-- Write your validity check here
+
+
+/-!
+If (whenever it's raining, the streets are wet), then (whenever the
+streets are wet it's raining.)
+-/
+def formal_5 : PLExpr := sorry
+
+
+/-!
+If (whever it's raining then bottom)/false, then (it's not raining).
+-/
+def formal_7  : PLExpr := sorry
+
+
+/-!
+If whenever it's raining the streets are wet, then whenever it's not
+raining the streets are not wet.
+-/
+def formal_8 : PLExpr := (rain ⇒ wet) ⇒ ((¬rain) ⇒ (¬wet))
+
+/-!
+If whenever it's raining the streets are wet, then whenever the
+streets are not wet, it's not be raining.
+-/
+def formal_9 : PLExpr := sorry
+
+
+/-!
+PROPOSITIONAL LOGIC TO ENGLISH: 50 points
+
+For each of the following propositions in propositional logic,
+open up some space after the proposition, in a comment block
+give a corresponding English-language form of that proposition;
+then *think* about whether the proposition is valid or not; and
+add a validity check using our validity checker. Finally, if
+a proposition is not valid, in English describe a case where
+the proposition is not true. Notice but don't worry (yet) about
+the funny names we assign to these propositions.
+-/
+
+def and_intro := sprink ⇒ rain ⇒ sprink ∧ rain
+def and_elim_left := sprink ∧ rain ⇒ sprink
+def and_elim_right := sprink ∧ rain ⇒ rain
+
+def or_intro_left := sprink ⇒ sprink ∨ rain
+def or_intro_right :=  rain ⇒ sprink ∨ rain
+def or_elim := rain ∨ sprink ⇒ (rain ⇒ wet) ⇒ (sprink ⇒ wet) ⇒ wet
+
+def not_intro := (sprink ⇒ ⊥) ⇒ ¬sprink
+def not_elim := ¬¬sprink ⇒ sprink
+
+def imp_intro := sprink ⇒ wet ⇒ (sprink ⇒ wet)
+def imp_elim := (sprink ⇒ wet) ⇒ sprink ⇒ wet
+
+def equiv_intro := (sprink ⇒ wet) ⇒ (wet ⇒ sprink) ⇒ (sprink ↔ wet)
+def equiv_elim_left := (sprink ↔ wet) ⇒ (sprink ⇒ wet)
+def equiv_elim_right := (sprink ↔ wet) ⇒ (wet ⇒ sprink)
+
+def affirm_disjunct := (wet ∨ sprink) ⇒ wet ⇒ ¬sprink
+def affirm_consequent := (sprink ⇒ wet) ⇒ wet ⇒ sprink
+def deny_antecedent := (sprink ⇒ wet) ⇒ ¬wet ⇒ ¬sprink
+
+end cs2120f24
