MyWork/natArithmetic/semantics.lean
@@ -1,0 +1,32 @@
+import «cs2120f24».Library.natArithmetic.syntax
+
+namespace cs2120f24.arith
+
+/-!
+Factorial function -- extra credit
+-/
+
+-- case analysis on constructors
+-- prefer Lean-provided notations
+def fac : Nat → Nat
+| 0 => 0                        -- Nat.zero
+| n' + 1 => (n' + 1) * fac n'   -- Nat.succ n'
+
+def unOpInterp : ArithUnOp → (Nat → Nat)
+| ArithUnOp.fac => fac
+
+def binOpInterp : ArithBinOp → (Nat → Nat → Nat)
+| ArithBinOp.add => Nat.add
+| ArithBinOp.sub => Nat.sub
+| ArithBinOp.mul => Nat.mul
+
+def arithVarInterp := ArithVar → Nat
+
+-- Semantics (incomplete, to be finished in homework)
+def arithEval : ArithExpr → arithVarInterp → Nat
+| ArithExpr.lit (fromNat : Nat),      i =>  fromNat
+| ArithExpr.var (fromVar : ArithVar), i => i fromVar
+| ArithExpr.unOp op e,                i => (unOpInterp op) (arithEval e i)
+| ArithExpr.binOp op e1 e2,           i => (binOpInterp op) (arithEval e1 i) (arithEval e2 i)
+
+end cs2120f24.arith
