MyWork/propLogicWithArith/semantics.lean
@@ -1,0 +1,29 @@
+import Cs2120f24.Library.propLogicWithArith.syntax
+
+namespace cs2120f24.arith
+
+/-!
+# Semantics
+-/
+
+def evalUnOp : UnOp → (Bool → Bool)
+| (UnOp.not) => not
+
+def evalBinOp : BinOp → (Bool → Bool → Bool)
+| BinOp.and => and
+| BinOp.or => or
+| BinOp.imp => imp
+| BinOp.iff => iff
+
+open PLExpr
+
+abbrev BoolInterp := BoolVar → Bool -- varInterp would be better name
+
+def evalPLExpr : PLExpr → BoolInterp → ArithVarInterp → Bool
+| lit_expr b,             _, _ => b
+| (var_expr v),           i, a => i v
+| (un_op_expr op e),      i, a => (evalUnOp op) (evalPLExpr e i a)
+| (bin_op_expr op e1 e2), i, a => (evalBinOp op) (evalPLExpr e1 i a) (evalPLExpr e2 i a)
+| arith_rel_expr e,       i, a => arithEval e a
+
+end cs2120f24.arith
